<?xml version="1.0"?>
<rdf:RDF xmlns="https://w3id.org/ontocis/topics#"
     xml:base="https://w3id.org/ontocis/topics"
     xmlns:rdf="http://www.w3.org/1999/02/22-rdf-syntax-ns#"
     xmlns:owl="http://www.w3.org/2002/07/owl#"
     xmlns:topics="https://w3id.org/ontocis/topics#"
     xmlns:xml="http://www.w3.org/XML/1998/namespace"
     xmlns:xsd="http://www.w3.org/2001/XMLSchema#"
     xmlns:skos="http://www.w3.org/2004/02/skos/core#"
     xmlns:dcterms="http://purl.org/dc/terms/#"
     xmlns:rdfs="http://www.w3.org/2000/01/rdf-schema#">
    <owl:Ontology rdf:about="https://w3id.org/ontocis/topics">
        <dcterms:license rdf:resource="https://opensource.org/licenses/MIT"/>
        <rdfs:label xml:lang="en">OntoCIS Topics</rdfs:label>
        <rdfs:comment xml:lang="en">Provides information about topics taught during a degree.</rdfs:comment>
        <rdfs:label xml:lang="es">OntoCIS Temas</rdfs:label>
        <rdfs:comment xml:lang="es">Brinda información sobre los temas que son dictados durante una carrera universitaria.</rdfs:comment>
    </owl:Ontology>



    <!--
    ///////////////////////////////////////////////////////////////////////////////////////
    //
    // Annotation properties
    //
    ///////////////////////////////////////////////////////////////////////////////////////
     -->




    <!-- https://w3id.org/ontocis/topics#altLabel -->

    <owl:AnnotationProperty rdf:about="https://w3id.org/ontocis/topics#altLabel">
        <rdfs:comment xml:lang="es">Agrega sinónimos, términos relacionados o variantes del término includo en la anotación rdfs:label.</rdfs:comment>
        <rdfs:comment xml:lang="en">Used for synoyms, related terms or different combinantions of the term that appears in the rdfs:label annotation.</rdfs:comment>
        <rdfs:label xml:lang="en">alternative label</rdfs:label>
        <rdfs:label xml:lang="es">etiqueta alternativa</rdfs:label>
    </owl:AnnotationProperty>





    <!--
    ///////////////////////////////////////////////////////////////////////////////////////
    //
    // Object Properties
    //
    ///////////////////////////////////////////////////////////////////////////////////////
     -->

     <!-- https://w3id.org/ontocis/topics#taughtIn -->

     <owl:ObjectProperty rdf:about="https://w3id.org/ontocis/topics#taughtIn">
         <rdfs:subPropertyOf rdf:resource="http://www.w3.org/2002/07/owl#topObjectProperty"/>
         <rdfs:domain rdf:resource="https://w3id.org/ontocis/topics#Topic"/>
         <rdfs:comment xml:lang="es">Indica que un tema se eseña o dicta durante una asignatura</rdfs:comment>
         <rdfs:comment xml:lang="en">It states that a topic is taught during a course</rdfs:comment>
         <rdfs:label xml:lang="es">enseñado en</rdfs:label>
         <rdfs:label xml:lang="en">taught in</rdfs:label>
     </owl:ObjectProperty>



    <!-- https://w3id.org/ontocis/topics#relatedTo -->

    <owl:ObjectProperty rdf:about="https://w3id.org/ontocis/topics#relatedTo">
        <rdfs:subPropertyOf rdf:resource="http://www.w3.org/2002/07/owl#topObjectProperty"/>
        <rdf:type rdf:resource="http://www.w3.org/2002/07/owl#SymmetricProperty"/>
        <rdfs:domain rdf:resource="https://w3id.org/ontocis/topics#Topic"/>
        <rdfs:range rdf:resource="https://w3id.org/ontocis/topics#Topic"/>
        <rdfs:comment xml:lang="es">Indica que un tema esta relacionado con otro tema</rdfs:comment>
        <rdfs:comment xml:lang="en">It states that a topic is related to another topic</rdfs:comment>
        <rdfs:label xml:lang="es">relacionado con</rdfs:label>
        <rdfs:label xml:lang="en">related to</rdfs:label>
    </owl:ObjectProperty>



    <!-- https://w3id.org/ontocis/topics#subtopicOf -->

    <owl:ObjectProperty rdf:about="https://w3id.org/ontocis/topics#subtopicOf">
        <rdfs:subPropertyOf rdf:resource="https://w3id.org/ontocis/topics#relatedTo"/>
        <rdf:type rdf:resource="http://www.w3.org/2002/07/owl#TransitiveProperty"/>
        <rdfs:domain rdf:resource="https://w3id.org/ontocis/topics#Topic"/>
        <rdfs:range rdf:resource="https://w3id.org/ontocis/topics#Topic"/>
        <rdfs:comment xml:lang="es">Indica que un tema es parte de otro tema más general</rdfs:comment>
        <rdfs:comment xml:lang="en">It states that a topic is part of a broader or more general topic</rdfs:comment>
        <rdfs:label xml:lang="es">subtema de</rdfs:label>
        <rdfs:label xml:lang="en">subtopic of</rdfs:label>
    </owl:ObjectProperty>



    <!--
    ///////////////////////////////////////////////////////////////////////////////////////
    //
    // Classes
    //
    ///////////////////////////////////////////////////////////////////////////////////////
     -->




    <!-- https://w3id.org/ontocis/topics#Topic -->

    <owl:Class rdf:about="https://w3id.org/ontocis/topics#Topic">
        <owl:equivalentClass rdf:resource="http://www.w3.org/2004/02/skos/core#Concept"/>
        <rdfs:comment xml:lang="en">A matter dealt with in a text, discourse, conversation, etc.</rdfs:comment>
        <rdfs:comment xml:lang="es">Asunto o materia sobre la que se trata en una conversación, un discurso, un escrito, etc.</rdfs:comment>
        <rdfs:label xml:lang="es">Tema</rdfs:label>
        <rdfs:label xml:lang="en">Topic</rdfs:label>
    </owl:Class>



    <!-- http://www.w3.org/2004/02/skos/core#Concept -->

    <owl:Class rdf:about="http://www.w3.org/2004/02/skos/core#Concept"/>
</rdf:RDF>



<!-- Generated by the OWL API (version 4.2.8.20170104-2310) https://github.com/owlcs/owlapi -->
